Publish previews: main c9dd9d40, 11 PRs
Main: c9dd9d40

Pull requests:
- PR #185: published at b7729749 (9 changed variants)
- PR #286: published at 89664253 (9 changed variants)
- PR #303: published at 70b26c1a (9 changed variants)
- PR #307: published at c3dcdd92 (9 changed variants)
- PR #319: published at 6406c730 (9 changed variants)
- PR #326: published at 10daf036 (9 changed variants)
- PR #345: published at 754a5aa5 (9 changed variants)
- PR #347: published at df57420e (9 changed variants)
- PR #349: published at 492b1d89 (9 changed variants)
- PR #351: published at d3ce5936 (9 changed variants)
- PR #352: published at 8327c16f (9 changed variants)

pr/356/head/lf/student/html/-verso-search/searchIndex_247.06e6aa64c2d4d338.js
@@ -1,1 +1,0 @@
-window.docContents[247].resolve({"/Postscript/#Postscript":{"contents":"Congratulations: We've reached the end of Logical Foundations!\n\n\n\n\n\n\n\n","context":"Logical Foundations","header":"12. Postscript","id":"/Postscript/#Postscript"}});
