pr/351/head/hl/solutions/lean/HL/Preface.lean
@@ -71,4 +71,4 @@ import SFLCompat
 --  Note to developers (Benjamin Pierce @bcpierce00):
 --      Other funding should be acknowledged here...
 
--- Built on 2026-08-31 21:54 UTC
+-- Built on 2026-09-02 14:27 UTC
