pr/351/head/hl/solutions/lean/HL/Slang.lean
@@ -446,7 +446,7 @@ scoped notation:55 e:56 " ⇓ " n:56 => EvalR e n
 --      think a simple `#print` may work as an alternative, assuming there
 --      are no namespace issues..
 
---  ### Exercise (1 star): beval_rules (Optional, manually graded) ⭐
+--  ### Exercise (1 star): beval_rules (Optional, Manually graded) ⭐
 
 --  Here, again, is the definition of the `Bexp.eval` function:
 --
@@ -680,4 +680,4 @@ end Slang.AevalRExtended
 --  switch between points of view at will -- exactly what we did above in
 --  `Slang.Aexp.evalR_iff_eval` and `Slang.Bexp.evalR_iff_eval`.
 
--- Built on 2026-08-31 21:54 UTC
+-- Built on 2026-09-02 14:27 UTC
