pr/351/head/hl/student/lean/HL/Equiv.lean
@@ -232,7 +232,7 @@ theorem while_false_equiv {b : Bexp} {c : Com} (hb : b.Equiv (bexp {false})) :
     apply EvalR.whileFalse
     simp [hb]
 
---  ### Exercise (2 stars): while_false_informal (Advanced, manually graded) ⭐⭐
+--  ### Exercise (2 stars): while_false_informal (Advanced, Manually graded) ⭐⭐
 
 --  Write an informal proof of `while_false_equiv`.
 
@@ -280,7 +280,7 @@ theorem while_true_nonterm {b : Bexp} {c : Com} {st st' : State} (hb : b.Equiv (
   | skip | asgn | seq | ifTrue | ifFalse =>
     contradiction -- heq says that different commands are equal
 
---  ### Exercise (2 stars): while_true_nonterm_informal (manually graded) ⭐⭐
+--  ### Exercise (2 stars): while_true_nonterm_informal (Manually graded) ⭐⭐
 
 --  Explain what the lemma `while_true_nonterm` means in English.
 
@@ -496,4 +496,4 @@ theorem Com.congruence.asgn {x : Ident} {a a' : Aexp} (ha : a.Equiv a') :
 --
 --  - (`<-`) Similar.
 
--- Built on 2026-08-31 21:54 UTC
+-- Built on 2026-09-02 14:27 UTC
