pr/351/head/lf/solutions/lean/LF/IndProp.lean
@@ -534,7 +534,7 @@ def Collatz' : Prop := ∀ (n : Nat), n ≠ 0 → CMS n 1
 --      HIDE: CH: Would it be helpful to add an exercise later proving CMS
 --      equivalent to CollatzHoldsFor?
 
---  ### Exercise (1 star): clos_refl_trans_sym (Optional, manually graded) ⭐
+--  ### Exercise (1 star): clos_refl_trans_sym (Optional, Manually graded) ⭐
 
 --  How would you modify the `ClosReflTrans` definition above so as to
 --  define the reflexive, symmetric, and transitive closure?
@@ -598,7 +598,7 @@ inductive Perm3 {α : Type} : List α → List α → Prop where
     (h₂₃ : Perm3 l₂ l₃) :
     Perm3 l₁ l₃
 
---  ### Exercise (1 star): perm (Optional, manually graded) ⭐
+--  ### Exercise (1 star): perm (Optional, Manually graded) ⭐
 
 --  According to this definition, is `[1, 2, 3]` a permutation of itself?
 
@@ -1628,7 +1628,7 @@ theorem ble_true_trans (n m k : Nat) :
   rw [ble_iff, ble_iff, ble_iff]
   apply le_trans
 
---  ### Exercise (3 stars): R_provability (manually graded) ⭐⭐⭐
+--  ### Exercise (3 stars): R_provability (Manually graded) ⭐⭐⭐
 
 --  We can define three-place relations, four-place relations, etc., in
 --  just the same way as binary relations. For example, consider the
@@ -1827,7 +1827,7 @@ theorem trans (l₁ l₂ l₃ : List Nat)
 
 end Subseq
 
---  ### Exercise (2 stars): R_provability2 (Optional, manually graded) ⭐⭐
+--  ### Exercise (2 stars): R_provability2 (Optional, Manually graded) ⭐⭐
 
 --  Suppose we give Lean the following definition:
 --
@@ -3080,4 +3080,4 @@ theorem pigeonhole_principle (α : Type) (l₁ l₂ : List α)
 --
 --  End Pigeon.
 
--- Built on 2026-08-31 21:53 UTC
+-- Built on 2026-09-02 14:26 UTC
