pr/351/head/lf/solutions/lean/LF/Preface.lean
@@ -436,4 +436,4 @@ import SFLCompat
 --  Note to developers (Benjamin Pierce @bcpierce00):
 --      Other funding should be acknowledged here...
 
--- Built on 2026-08-31 21:53 UTC
+-- Built on 2026-09-02 14:26 UTC
