pr/351/head/lf/solutions/lean/LF/Typeclasses.lean
@@ -1670,4 +1670,4 @@ example {α : Type} (x : α) [BEq α] [LawfulBEq α] (xs : List α)
 
 end Reflection
 
--- Built on 2026-08-31 21:53 UTC
+-- Built on 2026-09-02 14:26 UTC
