pr/351/head/lf/terse/lean/LF/Basics.lean
@@ -975,4 +975,4 @@ theorem and3_exchange (b c d : Bool) :
 
 end Nat
 
--- Built on 2026-08-31 21:53 UTC
+-- Built on 2026-09-02 14:26 UTC
