pr/351/head/lf/terse/lean/LF/Induction.lean
@@ -428,4 +428,4 @@ example (b : Bool) : (b || true) = true := by
 example (b c : Bool) : (b && c) = (c && b) := by
   cases b <;> cases c <;> rfl
 
--- Built on 2026-08-31 21:53 UTC
+-- Built on 2026-09-02 14:26 UTC
