pr/351/head/lf/terse/lean/LF/Postscript.lean
@@ -75,4 +75,4 @@ import SFLCompat
 --    develops formalized mathematics using Lean and
 --    Mathlib.
 
--- Built on 2026-08-31 21:53 UTC
+-- Built on 2026-09-02 14:26 UTC
