pr/351/head/ts/solutions/lean/TS/Smallstep.lean
@@ -1,4 +1,5 @@
 import TS.Slang
+import TS.AttributeDecls
 
 import SFLCompat
 
@@ -1508,4 +1509,94 @@ theorem compiler_is_correct (a : Aexp) :
 
 end Slang
 
--- Built on 2026-08-31 21:55 UTC
+--  ### Automation with `solve_by_elim`
+
+--  When experimenting with definitions of programming languages in Lean,
+--  we often want to see what a particular term steps to - i.e., we want to
+--  find proofs for goals of the form `t ⟶* t'`. Consider, for example,
+--  reducing an arithmetic expression using the small-step relation
+--  `AStep`.
+
+example : (.p (.c 3) (.p (.c 3) (.c 4))) ⟶* (.c 10) := by
+  apply Multi.step (y := .p (.c 3) (.c 7))
+  · apply Step.plusRight
+    · apply IsValue.const
+    · apply Step.plus
+  · apply Multi.step (y := .c 10)
+    · apply Step.plus
+    · apply Multi.refl
+
+--  Proofs that one term normalizes to another must repeatedly apply
+--  `Multi.step` until the term reaches a normal form, with some very
+--  simple intermediate steps along the way. Thankfully, we can automate
+--  this process with a new tactic: `solve_by_elim`. When supplied with a
+--  list of constructors, `solve_by_elim [c₁, c₂, c₃, ...]` will attempt to
+--  apply these constructors repeatedly to a goal. It will also
+--  automatically attempt to use simple tactics like `rfl`, `trivial`,
+--  `congr` and hypotheses from the context in order to solve simple goals.
+--  So, for example, the proof above also be written:
+
+example : (.p (.c 3) (.p (.c 3) (.c 4))) ⟶* (.c 10) := by
+  repeat apply Multi.step <;>
+    try solve_by_elim [Step.plusRight, Step.plusLeft, Step.plus, IsValue.const]
+
+--  This one script would suffice to prove most concrete reduction
+--  sequences for this simple language. To make it work for others, we
+--  would need to supply constructors for those other languages to
+--  `solve_by_elim`. The languages we will study in this book can grow to a
+--  large number of constructors for their `Step` relations, so we'd like a
+--  way to supply all of them to `solve_by_elim` more easily. Luckily, Lean
+--  supports this. We can register a constructor (or lemma) for use with
+--  `solve_by_elim` with an `attribute` command:
+
+--  THE FOLLOWING DETAILS CAN BE SKIPPED (Attributes)
+--  The command below tags all of these constructors with the `SimpleArith`
+--  attribute, which we can then use to automatically pull all of these
+--  constructors in when we use `solve_by_elim`. However, due to a
+--  limitation of Lean, this attribute needs to be pre-declared in a
+--  different file; we can't create it here and then immediately use it.
+--
+--  For this book, we've predeclared all the attributes we'll use in a file
+--  called `AttributeDecls.lean`, following the typical pattern from
+--  libraries like Mathlib.
+--  END DETAILS
+
+attribute [SimpleArith] Step.plusRight Step.plusLeft Step.plus IsValue.const
+
+--  This `using` option then tells `solve_by_elim` to try to use every
+--  constructor we've registered with the supplied attribute:
+
+example : (.p (.c 3) (.p (.c 3) (.c 4))) ⟶* (.c 10) := by
+  repeat apply Multi.step <;>
+    try solve_by_elim using SimpleArith
+
+--  We can package all this up into a dedicated tactic for solving
+--  reduction sequences, which we'll call `normalize`:
+
+syntax "normalize" " using " ident,+ : tactic
+
+macro_rules
+  | `(tactic| normalize using $xs,*) =>
+    `(tactic|
+      first
+      | apply Multi.refl
+      | (apply Multi.step
+         · solve_by_elim (maxDepth := 15) (constructor := false) only using $xs,*
+         · normalize using $xs,*))
+
+--  And voilà:
+
+example : (.p (.c 3) (.p (.c 3) (.c 4))) ⟶* (.c 10) := by
+  normalize using SimpleArith
+
+--  ### Exercise (1 star): normalize_ex ⭐
+
+--  Use the `normalize` tactic to prove the following. You will need to
+--  supply the term `e'` yourself.
+
+theorem normalize_ex : exists e', (.p (.c 3) (.p (.c 2) (.c 1))) ⟶* e' ∧ IsValue e' := by
+  exists (.c 6); constructor
+  · normalize using SimpleArith
+  · constructor
+
+-- Built on 2026-09-02 14:28 UTC
