pr/351/head/ts/student/lean/TS/StlcProp.lean
@@ -188,25 +188,43 @@ theorem progress' (t : Tm) (T : Ty) (hT : <{ ∅ ⊢ ~t ⦂ ~T }>) :
 --  context `Γ`. (Recall map inclusion, `Γ ⊆ Γ'`, from the `Typeclasses`
 --  chapter.)
 
--- IN PROGRESS
-theorem weakening (Γ Γ' : Context) (t : Tm) (T : Ty)
-    (hi : Γ ⊆ Γ') (hT : <{ ~Γ ⊢ ~t ⦂ ~T }>) : <{ ~Γ' ⊢ ~t ⦂ ~T }> := by
-  induction hT generalizing Γ' with
-  | var _ x _ h => exact .var _ x _ (hi h)
-  | abs _ x _ _ _ _ ih => exact .abs _ x _ _ _ (ih _ (PartialMap.update_subset _ _ _ _ hi))
-  | app _ _ _ _ _ _ _ ih₁ ih₂ => exact .app _ _ _ _ _ (ih₁ _ hi) (ih₂ _ hi)
-  | tru => exact .tru _
-  | fls => exact .fls _
-  | ite _ _ _ _ _ _ _ _ ih₁ ih₂ ih₃ => exact .ite _ _ _ _ _ (ih₁ _ hi) (ih₂ _ hi) (ih₃ _ hi)
+theorem weakening {Γ Γ' : Context} {t : Tm} {τ : Ty}
+    (hi : Γ ⊆ Γ') (ht : <{ ~Γ ⊢ ~t ⦂ ~τ }>) : <{ ~Γ' ⊢ ~t ⦂ ~τ }> := by
+  induction ht generalizing Γ' with
+  | var =>
+      constructor; apply hi; assumption
+  | abs _ _ _ _ _ _ ih =>
+      constructor; apply ih; apply PartialMap.update_subset; assumption
+  | app _ _ _ _ _ _ _ ih₁ ih₂ =>
+      constructor
+      . exact ih₁ hi
+      . exact ih₂ hi
+  | tru => constructor
+  | fls => constructor
+  | ite _ _ _ _ _ _ _ _ ih₁ ih₂ ih₃ =>
+      constructor
+      . exact ih₁ hi
+      . exact ih₂ hi
+      . exact ih₃ hi
+
+--  Through judicious use of `apply_rules`, we can heavily automate this
+--  proof. The tactic after `with` is applied to every case of the
+--  `induction` and handles all the cases using `apply_rules`'s automation.
+--  We must give the tactic access to all the `HasType` constructors and
+--  the `PartialMap.update_subset` lemma for this to work:
+
+theorem weakening' {Γ Γ' : Context} {t : Tm} {τ : Ty}
+    (hi : Γ ⊆ Γ') (ht : <{ ~Γ ⊢ ~t ⦂ ~τ }>) : <{ ~Γ' ⊢ ~t ⦂ ~τ }> := by
+  induction ht generalizing Γ' with (apply_rules [PartialMap.update_subset] using StlcTyping)
 
 --  The following simple corollary is what we actually need below.
 
-theorem weakening_empty (Γ : Context) (t : Tm) (T : Ty) (hT : <{ ∅ ⊢ ~t ⦂ ~T }>) :
-    <{ ~Γ ⊢ ~t ⦂ ~T }> :=
-  weakening _ _ _ _
-    (fun h => by
-      rw [PartialMap.getElem_empty] at h
-      cases h) hT
+theorem weakening_empty {Γ : Context} {t : Tm} {τ : Ty} (ht : <{ ∅ ⊢ ~t ⦂ ~τ }>) :
+    <{ ~Γ ⊢ ~t ⦂ ~τ }> := by
+  apply weakening _ ht
+  intro _ _ h
+  rw [PartialMap.getElem_empty] at h
+  contradiction
 
 --  ### The Substitution Lemma
 
@@ -238,7 +256,7 @@ theorem substitution_preserves_typing (Γ : Context) (x : String) (U : Ty)
         rw [subst_var_eq]
         have hUT : U = T := Option.some.inj h
         subst hUT
-        exact weakening_empty _ _ _ hv
+        exact weakening_empty hv
       · rw [PartialMap.update_neq hxy] at h
         rw [subst_var_ne _ _ _ hxy]
         exact .var _ y _ h
@@ -400,7 +418,7 @@ theorem preservation (t t' : Tm) (T : Ty)
 --    - Otherwise, `t` steps by `Step.ifStep`, and the desired conclusion
 --      follows directly from the first induction hypothesis.
 
---  ### Exercise (2 stars): subject_expansion_stlc (manually graded) ⭐⭐
+--  ### Exercise (2 stars): subject_expansion_stlc (Manually graded) ⭐⭐
 
 --  An exercise in the Types chapter asked about the *subject expansion*
 --  property for the simple language of arithmetic and boolean expressions.
@@ -620,7 +638,7 @@ theorem context_invariance (Γ Γ' : Context) (t : Tm) (T : Ty)
 --  theorems for the simply typed lambda-calculus (as Lean theorems). You
 --  can write `sorry` for the proofs.
 
---  ### Exercise (2 stars): stlc_variation1 (manually graded) ⭐⭐
+--  ### Exercise (2 stars): stlc_variation1 (Manually graded) ⭐⭐
 
 --  Suppose we add a new term `zap` with the following reduction rule
 --
@@ -642,7 +660,7 @@ theorem context_invariance (Γ Γ' : Context) (t : Tm) (T : Ty)
 --
 --  - Preservation
 
---  ### Exercise (2 stars): stlc_variation2 (manually graded) ⭐⭐
+--  ### Exercise (2 stars): stlc_variation2 (Manually graded) ⭐⭐
 
 --  Suppose instead that we add a new term `foo` with the following
 --  reduction rules:
@@ -664,7 +682,7 @@ theorem context_invariance (Γ Γ' : Context) (t : Tm) (T : Ty)
 --
 --  - Preservation
 
---  ### Exercise (2 stars): stlc_variation3 (manually graded) ⭐⭐
+--  ### Exercise (2 stars): stlc_variation3 (Manually graded) ⭐⭐
 
 --  Suppose instead that we remove the rule `Step.app1` from the `step`
 --  relation. Which of the following properties of the STLC remain true in
@@ -1205,4 +1223,4 @@ theorem progress (t : Tm) (T : Ty) (hT : <{ ∅ ⊢ ~t ⦂ ~T }>) :
 
 end StlcArith
 
--- Built on 2026-08-31 21:55 UTC
+-- Built on 2026-09-02 14:28 UTC
