pr/351/head/ts/terse/lean/TS/Types.lean
@@ -764,7 +764,7 @@ end TM
 --  breaks. (These are graded manually; there is no Lean
 --  code to complete.)
 
---  ### Exercise (2 stars): variation1 (manually graded) ⭐⭐
+--  ### Exercise (2 stars): variation1 (Manually graded) ⭐⭐
 
 --  Suppose that we add this new rule to the typing
 --  relation:
@@ -780,7 +780,7 @@ end TM
 --  - Progress
 --  - Preservation
 
---  ### Exercise (2 stars): variation2 (manually graded) ⭐⭐
+--  ### Exercise (2 stars): variation2 (Manually graded) ⭐⭐
 
 --  Suppose, instead, that we add this new rule to the
 --  `Tm.Step` relation:
@@ -839,7 +839,7 @@ end TM
 --  definitions that break just one of the properties and
 --  leave the others alone.
 
---  ### Exercise (1 star): remove_pred0 (manually graded) ⭐
+--  ### Exercise (1 star): remove_pred0 (Manually graded) ⭐
 
 --  The reduction rule `predZero` is a bit
 --  counter-intuitive: we might feel that it makes more
@@ -848,7 +848,7 @@ end TM
 --  by removing the rule from the definition of `Tm.Step`?
 --  Would doing so create any problems elsewhere?
 
---  ### Exercise (4 stars): prog_pres_bigstep (Advanced, manually graded) ⭐⭐⭐⭐
+--  ### Exercise (4 stars): prog_pres_bigstep (Advanced, Manually graded) ⭐⭐⭐⭐
 
 --  Suppose our evaluation relation is defined in the
 --  big-step style. State appropriate analogs of the
@@ -860,4 +860,4 @@ end TM
 --  Why might we prefer the small-step semantics for stating
 --  preservation and progress?
 
--- Built on 2026-08-31 21:55 UTC
+-- Built on 2026-09-02 14:28 UTC
